share/steel/examples/pulse/lib/Pulse.Lib.Invariants.fsti
@@ -1,0 +1,25 @@
+module Pulse.Lib.Invariants
+
+open Pulse.Lib.Core
+
+val inv (p:vprop) : Type
+
+(* Does this have to be decidable? *)
+val mem_inv (#p:vprop) : inames -> inv p -> Ghost.erased bool
+
+val add_inv (#p:vprop) : inames -> inv p -> inames
+
+// THIS SHOULD BE stt_unobservable
+
+val new_invariant (p:vprop)
+  : stt_ghost (inv p) emp_inames p (fun _ -> emp)
+  
+val with_invariant
+  (#p:vprop)
+  (#a : Type)
+  (#pre : vprop)
+  (#post : a -> vprop)
+  (#opened : inames)
+  (i : inv p{not (mem_inv opened i)})
+  (f : unit -> stt_ghost a opened (p ** pre) (fun x -> p ** post x))
+  : stt_ghost a (add_inv opened i) pre post
